src/Lustre/LTyping.v
@@ -26,23 +26,23 @@ Module Type LTYPING
        (Import Op   : OPERATORS)
        (Import Syn  : LSYNTAX Ids Op).
 
+  Inductive wt_clock : list (ident * type) -> clock -> Prop :=
+  | wt_Cbase: forall vars,
+      wt_clock vars Cbase
+  | wt_Con: forall vars ck x b,
+      In (x, bool_type) vars ->
+      wt_clock vars ck ->
+      wt_clock vars (Con ck x b).
+
+  Inductive wt_nclock : list (ident * type) -> nclock -> Prop :=
+  | wt_Cnamed: forall vars id ck,
+      wt_clock vars ck ->
+      wt_nclock vars (ck, id).
+
   Section WellTyped.
 
     Variable G    : global.
     Variable vars : list (ident * type).
-
-    Inductive wt_clock : clock -> Prop :=
-    | wt_Cbase:
-        wt_clock Cbase
-    | wt_Con: forall ck x b,
-        In (x, bool_type) vars ->
-        wt_clock ck ->
-        wt_clock (Con ck x b).
-
-    Inductive wt_nclock : nclock -> Prop :=
-    | wt_Cnamed: forall id ck,
-        wt_clock ck ->
-        wt_nclock (ck, id).
 
     Inductive wt_exp : exp -> Prop :=
     | wt_Econst: forall c,
@@ -50,14 +50,14 @@ Module Type LTYPING
 
     | wt_Evar: forall x ty nck,
         In (x, ty) vars ->
-        wt_nclock nck ->
+        wt_nclock vars nck ->
         wt_exp (Evar x (ty, nck))
 
     | wt_Eunop: forall op e tye ty nck,
         wt_exp e ->
         typeof e = [tye] ->
         type_unop op tye = Some ty ->
-        wt_nclock nck ->
+        wt_nclock vars nck ->
         wt_exp (Eunop op e (ty, nck))
 
     | wt_Ebinop: forall op e1 e2 ty1 ty2 ty nck,
@@ -66,7 +66,7 @@ Module Type LTYPING
         typeof e1 = [ty1] ->
         typeof e2 = [ty2] ->
         type_binop op ty1 ty2 = Some ty ->
-        wt_nclock nck ->
+        wt_nclock vars nck ->
         wt_exp (Ebinop op e1 e2 (ty, nck))
 
     | wt_Efby: forall e0s es anns,
@@ -74,14 +74,14 @@ Module Type LTYPING
         Forall wt_exp es ->
         typesof es = map fst anns ->
         typesof e0s = map fst anns ->
-        Forall wt_nclock (map snd anns) ->
+        Forall (wt_nclock vars) (map snd anns) ->
         wt_exp (Efby e0s es anns)
 
     | wt_Ewhen: forall es x b tys nck,
         Forall wt_exp es ->
         typesof es = tys ->
         In (x, bool_type) vars ->
-        wt_nclock nck ->
+        wt_nclock vars nck ->
         wt_exp (Ewhen es x b (tys, nck))
 
     | wt_Emerge: forall x ets efs tys nck,
@@ -90,7 +90,7 @@ Module Type LTYPING
         In (x, bool_type) vars ->
         typesof ets = tys ->
         typesof efs = tys ->
-        wt_nclock nck ->
+        wt_nclock vars nck ->
         wt_exp (Emerge x ets efs (tys, nck))
 
     | wt_Eifte: forall e ets efs tys nck,
@@ -100,7 +100,7 @@ Module Type LTYPING
         typeof e = [bool_type] ->
         typesof ets = tys ->
         typesof efs = tys ->
-        wt_nclock nck ->
+        wt_nclock vars nck ->
         wt_exp (Eite e ets efs (tys, nck))
 
     | wt_Eapp: forall f es anns n,
@@ -108,7 +108,7 @@ Module Type LTYPING
         find_node f G = Some n ->
         Forall2 (fun et '(_, (t, _)) => et = t) (typesof es) n.(n_in) ->
         Forall2 (fun a '(_, (t, _)) => fst a = t) anns n.(n_out) ->
-        Forall (fun a => wt_nclock (snd a)) anns ->
+        Forall (fun a => wt_nclock (vars++(idty (fresh_ins es++anon_streams anns))) (snd a)) anns ->
         wt_exp (Eapp f es None anns)
 
     | wt_EappReset: forall f es r anns n,
@@ -116,7 +116,7 @@ Module Type LTYPING
         find_node f G = Some n ->
         Forall2 (fun et '(_, (t, _)) => et = t) (typesof es) n.(n_in) ->
         Forall2 (fun a '(_, (t, _)) => fst a = t) anns n.(n_out) ->
-        Forall (fun a => wt_nclock (snd a)) anns ->
+        Forall (fun a => wt_nclock (vars++(idty (fresh_ins es++anon_streams anns))) (snd a)) anns ->
         wt_exp r ->
         typeof r = [bool_type] ->
         wt_exp (Eapp f es (Some r) anns).
@@ -132,7 +132,7 @@ Module Type LTYPING
       Hypothesis EvarCase:
         forall x ty nck,
           In (x, ty) vars ->
-          wt_nclock nck ->
+          wt_nclock vars nck ->
           P (Evar x (ty, nck)).
 
       Hypothesis EunopCase:
@@ -141,7 +141,7 @@ Module Type LTYPING
           P e ->
           typeof e = [tye] ->
           type_unop op tye = Some ty ->
-          wt_nclock nck ->
+          wt_nclock vars nck ->
           P (Eunop op e (ty, nck)).
 
       Hypothesis EbinopCase:
@@ -153,7 +153,7 @@ Module Type LTYPING
           typeof e1 = [ty1] ->
           typeof e2 = [ty2] ->
           type_binop op ty1 ty2 = Some ty ->
-          wt_nclock nck ->
+          wt_nclock vars nck ->
           P (Ebinop op e1 e2 (ty, nck)).
 
       Hypothesis EfbyCase:
@@ -164,7 +164,7 @@ Module Type LTYPING
           Forall P es ->
           typesof es = map fst anns ->
           typesof e0s = map fst anns ->
-          Forall wt_nclock (map snd anns) ->
+          Forall (wt_nclock vars) (map snd anns) ->
           P (Efby e0s es anns).
 
       Hypothesis EwhenCase:
@@ -173,7 +173,7 @@ Module Type LTYPING
           Forall P es ->
           typesof es = tys ->
           In (x, bool_type) vars ->
-          wt_nclock nck ->
+          wt_nclock vars nck ->
           P (Ewhen es x b (tys, nck)).
 
       Hypothesis EmergeCase:
@@ -185,7 +185,7 @@ Module Type LTYPING
           In (x, bool_type) vars ->
           typesof ets = tys ->
           typesof efs = tys ->
-          wt_nclock nck ->
+          wt_nclock vars nck ->
           P (Emerge x ets efs (tys, nck)).
 
       Hypothesis EiteCase:
@@ -199,7 +199,7 @@ Module Type LTYPING
           typeof e = [bool_type] ->
           typesof ets = tys ->
           typesof efs = tys ->
-          wt_nclock nck ->
+          wt_nclock vars nck ->
           P (Eite e ets efs (tys, nck)).
 
       Hypothesis EappCase:
@@ -209,7 +209,7 @@ Module Type LTYPING
           find_node f G = Some n ->
           Forall2 (fun et '(_, (t, _)) => et = t) (typesof es) n.(n_in) ->
           Forall2 (fun a '(_, (t, _)) => fst a = t) anns n.(n_out) ->
-          Forall (fun a => wt_nclock (snd a)) anns ->
+          Forall (fun a => wt_nclock (vars++(idty (fresh_ins es++anon_streams anns))) (snd a)) anns ->
           P (Eapp f es None anns).
 
       Hypothesis EappResetCase:
@@ -219,7 +219,7 @@ Module Type LTYPING
           find_node f G = Some n ->
           Forall2 (fun et '(_, (t, _)) => et = t) (typesof es) n.(n_in) ->
           Forall2 (fun a '(_, (t, _)) => fst a = t) anns n.(n_out) ->
-          Forall (fun a => wt_nclock (snd a)) anns ->
+          Forall (fun a => wt_nclock (vars++(idty (fresh_ins es++anon_streams anns))) (snd a)) anns ->
           wt_exp r ->
           P r ->
           typeof r = [bool_type] ->
@@ -240,9 +240,9 @@ Module Type LTYPING
           clear H3. induction H0; auto.
           clear H4. induction H1; auto.
         - eapply EappCase; eauto.
-          clear H1. induction H; eauto.
+          clear H1 H3. induction H; eauto.
         - eapply EappResetCase; eauto.
-          clear H1. induction H; eauto.
+          clear H1 H3. induction H; eauto.
       Qed.
 
     End wt_exp_ind2.
@@ -262,8 +262,7 @@ Module Type LTYPING
     :=    wt_clocks n.(n_in) n.(n_in)
        /\ wt_clocks (n.(n_in) ++ n.(n_out)) n.(n_out)
        /\ wt_clocks (n.(n_in) ++ n.(n_out) ++ n.(n_vars)) n.(n_vars)
-       /\ Forall (wt_equation G (idty (n.(n_in) ++ n.(n_vars) ++ n.(n_out))))
-                 n.(n_eqs).
+       /\ Forall (wt_equation G (idty (n.(n_in) ++ n.(n_vars) ++ n.(n_out)))) n.(n_eqs).
 
   Inductive wt_global : global -> Prop :=
   | wtg_nil:
@@ -372,9 +371,9 @@ Module Type LTYPING
       induction H using wt_exp_ind2;
       (rewrite Henv in * || rewrite <-Henv in * || idtac);
       try match goal with
-          | H:Forall (fun a => wt_nclock env' (snd a)) _ |- _ =>
+          | H:Forall (fun a => wt_nclock (env' ++ _) (snd a)) _ |- _ =>
             setoid_rewrite Henv in H
-          | H:Forall (fun a => wt_nclock env (snd a)) _ |- _ =>
+          | H:Forall (fun a => wt_nclock (env ++ _) (snd a)) _ |- _ =>
             setoid_rewrite <-Henv in H
           end;
       eauto with ltyping;
@@ -412,364 +411,59 @@ Module Type LTYPING
       now rewrite <-Henv in Hin.
   Qed.
 
-  Lemma wt_exp_clockof:
-    forall G env e,
-      wt_exp G env e ->
-      Forall (wt_clock env) (clockof e).
-  Proof.
-    intros * Hwt.
-    apply Forall_forall. intros ck Hin.
-    inv Hwt; simpl in *.
-    - destruct Hin as [Hin|]; [|contradiction].
-      rewrite <-Hin; auto with ltyping.
-    - destruct Hin as [Hin|]; [|contradiction].
-      rewrite <-Hin.
-      destruct nck; unfold clock_of_nclock; simpl in *;
-        match goal with H:wt_nclock _ _ |- _ => inv H end; auto.
-    - destruct Hin as [Hin|]; [|contradiction].
-      rewrite <-Hin.
-      destruct nck; unfold clock_of_nclock; simpl in *;
-        match goal with H:wt_nclock _ _ |- _ => inv H end; auto.
-    - destruct Hin as [Hin|]; [|contradiction].
-      rewrite <-Hin.
-      destruct nck; unfold clock_of_nclock; simpl in *;
-        match goal with H:wt_nclock _ _ |- _ => inv H end; auto.
-    - match goal with H:Forall (wt_nclock _) _ |- _ =>
-                      rewrite Forall_map in H end.
-      apply in_map_iff in Hin.
-      destruct Hin as ((ty & nck) & Hck & Hin).
-      apply Forall_forall with (1:=H3) in Hin.
-      destruct nck; unfold clock_of_nclock in *; simpl in *; subst;
-        match goal with H:wt_nclock _ _ |- _ => inv H end; auto.
-    - destruct nck; unfold clock_of_nclock in *; simpl in *;
-        apply in_map_iff in Hin; destruct Hin as (? & Hs & Hin); subst;
-          match goal with H:wt_nclock _ _ |- _ => inv H end; auto.
-    - destruct nck; unfold clock_of_nclock in *; simpl in *;
-        apply in_map_iff in Hin; destruct Hin as (? & Hs & Hin); subst;
-          match goal with H:wt_nclock _ _ |- _ => inv H end; auto.
-    - destruct nck; unfold clock_of_nclock in *; simpl in *;
-        apply in_map_iff in Hin; destruct Hin as (? & Hs & Hin); subst;
-          match goal with H:wt_nclock _ _ |- _ => inv H end; auto.
-    - apply in_map_iff in Hin.
-      destruct Hin as (x & Hs & Hin).
-      match goal with H:Forall _ anns |- _ =>
-                      apply Forall_forall with (1:=H) in Hin end.
-      destruct x as (ty, nck).
-      destruct nck; unfold clock_of_nclock in *; simpl in *;
-        subst; match goal with H:wt_nclock _ _ |- _ => inv H end; auto.
-    - apply in_map_iff in Hin.
-      destruct Hin as (x & Hs & Hin).
-      match goal with H:Forall _ anns |- _ =>
-                      apply Forall_forall with (1:=H) in Hin end.
-      destruct x as (ty, nck).
-      destruct nck; unfold clock_of_nclock in *; simpl in *;
-        subst; match goal with H:wt_nclock _ _ |- _ => inv H end; auto.
-  Qed.
-
-  (** Validation *)
-
-  Module OpAux := OperatorsAux Op.
-
-  Section ValidateExpression.
-
-    Variable G : global.
-    Variable venv : Env.t (type * clock).
-
-    Open Scope option_monad_scope.
-
-    Fixpoint check_clock (ck : clock) : bool :=
-      match ck with
-      | Cbase => true
-      | Con ck' x b =>
-        match Env.find x venv with
-        | None => false
-        | Some (xt, _) => (xt ==b bool_type) && check_clock ck'
-        end
-      end.
-
-    Definition check_nclock (nck : nclock) : bool :=
-      check_clock (fst nck).
-
-    Definition check_paired_types (t1 t2 : type) (tc : ann) : bool :=
-      let '(t, c) := tc in
-      (t1 ==b t) && (t2 ==b t) && (check_nclock c).
-
-    Definition check_reset (rt : option (option (list type))) : bool :=
-      match rt with
-      | None => true
-      | Some (Some [ty]) => ty ==b bool_type
-      | _ => false
-      end.
-
-    Function check_var (x : ident) (ty : type) : bool :=
-      match Env.find x venv with
-      | None => false
-      | Some (xt, _) => ty ==b xt
-      end.
-
-    Fixpoint check_exp (e : exp) : option (list type) :=
-      match e with
-      | Econst c => Some ([type_const c])
-
-      | Evar x (xt, nck) =>
-        if check_var x xt && check_nclock nck then Some [xt] else None
-
-      | Eunop op e (xt, nck) =>
-        do te <- assert_singleton (check_exp e);
-        do t <- type_unop op te;
-        if (xt ==b t) && check_nclock nck then Some [xt] else None
-
-      | Ebinop op e1 e2 (xt, nck) =>
-        do te1 <- assert_singleton (check_exp e1);
-        do te2 <- assert_singleton (check_exp e2);
-        do t <- type_binop op te1 te2;
-        if (xt ==b t) && check_nclock nck then Some [xt] else None
-
-      | Efby e0s es anns =>
-        do t0s <- oconcat (map check_exp e0s);
-        do ts <- oconcat (map check_exp es);
-        if forall3b check_paired_types t0s ts anns
-        then Some (map fst anns) else None
-
-      | Ewhen es x b (tys, nck) =>
-        do ts <- oconcat (map check_exp es);
-        if check_var x bool_type && (forall2b equiv_decb ts tys) && (check_nclock nck)
-        then Some tys else None
-
-      | Emerge x e1s e2s (tys, nck) =>
-        do t1s <- oconcat (map check_exp e1s);
-        do t2s <- oconcat (map check_exp e2s);
-        if check_var x bool_type
-             && (forall3b equiv_decb3 t1s t2s tys)
-             && (check_nclock nck)
-        then Some tys else None
-
-      | Eite e e1s e2s (tys, nck) =>
-        do t1s <- oconcat (map check_exp e1s);
-        do t2s <- oconcat (map check_exp e2s);
-        do xt <- assert_singleton (check_exp e);
-        if (xt ==b bool_type)
-             && (forall3b equiv_decb3 t1s t2s tys)
-             && (check_nclock nck)
-        then Some tys else None
-
-      | Eapp f es ro anns =>
-        do n <- find_node f G;
-        do ts <- oconcat (map check_exp es);
-        if (forall2b (fun et '(_, (t, _)) => et ==b t) ts n.(n_in))
-             && (forall2b (fun '(ot, oc) '(_, (t, _)) =>
-                             check_nclock oc && (ot ==b t)) anns n.(n_out))
-             && check_reset (option_map check_exp ro)
-        then Some (map fst anns)
-        else None
-      end.
-
-    Definition check_equation (eq : equation) : bool :=
-      let '(xs, es) := eq in
-      match oconcat (map check_exp es) with
-      | None => false
-      | Some tys => forall2b check_var xs tys
-      end.
-
-    (* TODO: Move elsewhere? *)
-    Local Ltac DestructMatch :=
-      repeat progress
-             match goal with
-             | H:match ?e with _ => _ end = _ |- _ =>
-               let Heq := fresh "Heq" in
-               destruct e eqn:Heq; try discriminate
-             end.
-
-    Lemma check_clock_correct:
-      forall ck,
-        check_clock ck = true ->
-        wt_clock (idty (Env.elements venv)) ck.
-    Proof.
-      induction ck; intro CC. now constructor.
-      simpl in CC. DestructMatch.
-      rewrite Bool.andb_true_iff in CC; destruct CC as (CC1 & CC2).
-      apply IHck in CC2. rewrite equiv_decb_equiv in CC1; inv CC1.
-      apply Env.elements_correct in Heq.
-      constructor; auto. apply In_idty_exists; eauto.
-    Qed.
-
-    Lemma check_nclock_correct:
-      forall nck,
-        check_nclock nck = true ->
-        wt_nclock (idty (Env.elements venv)) nck.
-    Proof.
-      destruct nck as (n, ck).
-      intro CC; now apply check_clock_correct in CC.
-    Qed.
-
-    (* TODO: add to a database *)
-    Hint Extern 2 (In _ (idty _)) => apply In_idty_exists.
-
-    Lemma check_var_correct:
-      forall x ty,
-        check_var x ty = true <-> In (x, ty) (idty (Env.elements venv)).
-    Proof.
-      unfold check_var. split; intros HH.
-      - DestructMatch; simpl.
-        rewrite equiv_decb_equiv in HH. inv HH.
-        take (Env.find _ _ = Some _) and apply Env.elements_correct in it; eauto.
-      - apply In_idty_exists in HH as (ck & HH).
-        apply Env.elements_complete in HH as ->.
-        apply equiv_decb_refl.
-    Qed.
-
-    Lemma check_paired_types_correct:
-      forall tys1 tys2 anns,
-        forall3b check_paired_types tys1 tys2 anns = true ->
-        tys1 = map fst anns
-        /\ tys2 = map fst anns
-        /\ Forall (wt_nclock (idty (Env.elements venv))) (map snd anns).
-    Proof.
-      setoid_rewrite forall3b_Forall3.
-      induction 1 as [|ty1 ty2 (ty, nck) tys1 tys2 anns IH1 IH2 (? & ? & IH3)];
-        subst; simpl; eauto.
-      simpl in IH1.
-      repeat rewrite Bool.andb_true_iff in IH1.
-      setoid_rewrite equiv_decb_equiv in IH1.
-      destruct IH1 as ((-> & ->) & IH1).
-      apply check_nclock_correct in IH1. auto.
-    Qed.
-
-    Lemma oconcat_map_check_exp':
-      forall {f} es tys,
-        (forall e tys,
-            In e es ->
-            f e = Some tys ->
-            wt_exp G (idty (Env.elements venv)) e /\ typeof e = tys) ->
-        oconcat (map f es) = Some tys ->
-        Forall (wt_exp G (idty (Env.elements venv))) es
-        /\ typesof es = tys.
-    Proof.
-      induction es as [|e es IH]; intros tys WTf CE. now inv CE; auto.
-      simpl in CE. destruct (f e) eqn:Ce; [|now omonadInv CE].
-      destruct (oconcat (map f es)) as [tes|]; [|now omonadInv CE].
-      omonadInv CE. simpl.
-      apply WTf in Ce as (Ce1 & ->); auto with datatypes.
-      destruct (IH tes) as (? & ->); auto.
-      intros * Ies Fe. apply WTf in Fe; auto with datatypes.
-    Qed.
-
-    Lemma check_exp_correct:
-      forall e tys,
-        check_exp e = Some tys ->
-        wt_exp G (idty (Env.elements venv)) e
-        /\ typeof e = tys.
-    Proof.
-      induction e using exp_ind2; simpl; intros tys CE;
-      repeat progress
-               match goal with
-               | a:ann |- _ => destruct a
-               | a:lann |- _ => destruct a
-               | p:type * clock |- _ => destruct p
-               | H:obind _ _ = Some _ |- _ => omonadInv H
-               | H:obind2 _ _ = Some _ |- _ => omonadInv H
-               | H:obind ?v _ = Some _ |- _ =>
-                 let OE:=fresh "OE0" in destruct v eqn:OE; [simpl in H|now omonadInv H]
-               | H: _ && _ = true |- _ => apply Bool.andb_true_iff in H as (? & ?)
-               | H: ((_ ==b _) = true) |- _ => rewrite equiv_decb_equiv in H; inv H
-               | H: check_nclock _ = true |- _ => apply check_nclock_correct in H
-               | H: Env.find _ _ = Some _ |- _ => apply Env.elements_correct in H
-               | H:(obind2 (Env.find ?x ?env) _) = Some _ |- _ =>
-                 let EF := fresh "EF0" in
-                 destruct (Env.find x env) eqn:EF
-               | H:(if ?c then Some _ else None) = Some _ |- _ =>
-                 let C := fresh "C0" in
-                 destruct c eqn:C
-               | H:None = Some _ |- _ => discriminate
-               | H:Some _ = Some _ |- _ => inv H
-               | H:assert_singleton _ = Some _ |- _ => apply assert_singleton_spec in H
-               | H:check_var _ _ = true |- _ => apply check_var_correct in H
-               | H:forall3b check_paired_types ?tys1 ?tys2 ?anns = true |- _ =>
-                 apply check_paired_types_correct in H as (? & ? & ?)
-               | H:forall2b equiv_decb ?xs ?ys = true |- _ =>
-                 apply forall2b_Forall2_equiv_decb in H
-               | H:forall3b equiv_decb3 _ _ _ = true |- _ =>
-                 apply forall3b_equiv_decb3 in H as (? & ?)
-               | H:Forall2 eq _ _ |- _ => apply Forall2_eq in H
-               | H:forall2b _ _ _ = true |- _ => apply forall2b_Forall2 in H
-               end.
-      - (* Econst *)
-        eauto using wt_exp.
-      - (* Evar *)
-        eauto using wt_exp.
-      - (* Eunop *)
-        apply IHe in OE0 as (? & ?). eauto using wt_exp.
-      - (* Ebinop *)
-        apply IHe1 in OE0 as (? & ?); apply IHe2 in OE1 as (? & ?).
-        eauto using wt_exp.
-      - (* Efby *)
-        take (Forall _ e0s) and rewrite Forall_forall in it.
-        take (Forall _ es) and rewrite Forall_forall in it.
-        apply oconcat_map_check_exp' in OE0 as (? & ?); auto.
-        apply oconcat_map_check_exp' in OE1 as (? & ?); auto.
-        subst; eauto using wt_exp.
-      - (* Ewhen *)
-        subst. take (Forall _ es) and rewrite Forall_forall in it.
-        take (oconcat (map check_exp _) = Some _) and
-             apply oconcat_map_check_exp' in it as (? & ?); eauto using wt_exp.
-      - (* Emerge *)
-        take (Forall _ ets) and rewrite Forall_forall in it.
-        take (Forall _ efs) and rewrite Forall_forall in it.
-        repeat take (oconcat (map check_exp _) = Some _) and
-               apply oconcat_map_check_exp' in it as (? & ?); auto.
-        subst. eauto using wt_exp.
-      - (* Eite *)
-        take (check_exp _ = Some _) and apply IHe in it as (? & ?).
-        take (Forall _ ets) and rewrite Forall_forall in it.
-        take (Forall _ efs) and rewrite Forall_forall in it.
-        repeat take (oconcat (map check_exp _) = Some _) and
-               apply oconcat_map_check_exp' in it as (? & ?); auto.
-        subst. eauto using wt_exp.
-      - (* Eapp *)
-        take (Forall _ es) and rewrite Forall_forall in it.
-        take (oconcat (map check_exp _) = Some _) and
-             apply oconcat_map_check_exp' in it as (? & ?); auto.
-        split; auto. subst.
-        assert (Forall2 (fun et '(_, (t, _)) => et = t) (typesof es) n.(n_in)).
-        { take (Forall2 _ (typesof es) n.(n_in))
-               and apply Forall2_impl_In with (2:=it).
-          intros ? (? & (? & ?)) ? ? EQ.
-          now rewrite equiv_decb_equiv in EQ. }
-        assert (Forall2 (fun ann '(_, (t, _)) => fst ann = t) a n.(n_out)).
-        { take (Forall2 _ _ n.(n_out)) and apply Forall2_impl_In with (2:=it).
-          intros (? & ?) (? & (? & ?)) ? ? EQ.
-          apply Bool.andb_true_iff in EQ as (EQ1 & EQ2).
-          now rewrite equiv_decb_equiv in EQ2. }
-        assert (Forall (fun ann => wt_nclock (idty (Env.elements venv)) (snd ann)) a).
-        { repeat take (Forall2 _ _ n.(n_out)) and apply Forall2_ignore2 in it.
-          apply Forall_impl_In with (2:=it).
-          intros (? & ?) ? ((? & (? & ?)) & (? & EQ)).
-          apply Bool.andb_true_iff in EQ as (EQ1 & EQ2).
-          apply check_nclock_correct with (1:=EQ1). }
-        destruct ro; econstructor; eauto; simpl in *;
-          take (forall tys, check_exp _ = Some tys -> _ /\ _) and rename it into CE;
-          DestructMatch; subst; specialize (CE _ eq_refl) as (CE1 & CE2); auto.
-        rewrite CE2.
-        now take ((_ ==b _) = true) and rewrite equiv_decb_equiv in it; inv it.
-    Qed.
-
-    Lemma check_equation_correct:
-      forall eq,
-        check_equation eq = true ->
-        wt_equation G (idty (Env.elements venv)) eq.
-    Proof.
-      intros eq CE. destruct eq as (xs, es); simpl in CE.
-      DestructMatch.
-      take (oconcat (map check_exp _) = Some _)
-           and apply oconcat_map_check_exp' in it as (? & ?).
-      2:now intros; apply check_exp_correct.
-      take (forall2b check_var _ _ = true)
-           and apply forall2b_Forall2 in it.
-      setoid_rewrite check_var_correct in it.
-      subst; constructor; auto.
-    Qed.
-
-  End ValidateExpression.
+  (* Lemma wt_exp_clockof: *)
+  (*   forall G env e, *)
+  (*     wt_exp G env e -> *)
+  (*     Forall (wt_clock env) (clockof e). *)
+  (* Proof. *)
+  (*   intros * Hwt. *)
+  (*   apply Forall_forall. intros ck Hin. *)
+  (*   inv Hwt; simpl in *. *)
+  (*   - destruct Hin as [Hin|]; [|contradiction]. *)
+  (*     rewrite <-Hin; auto with ltyping. *)
+  (*   - destruct Hin as [Hin|]; [|contradiction]. *)
+  (*     rewrite <-Hin. *)
+  (*     destruct nck; unfold clock_of_nclock; simpl in *; *)
+  (*       match goal with H:wt_nclock _ _ |- _ => inv H end; auto. *)
+  (*   - destruct Hin as [Hin|]; [|contradiction]. *)
+  (*     rewrite <-Hin. *)
+  (*     destruct nck; unfold clock_of_nclock; simpl in *; *)
+  (*       match goal with H:wt_nclock _ _ |- _ => inv H end; auto. *)
+  (*   - destruct Hin as [Hin|]; [|contradiction]. *)
+  (*     rewrite <-Hin. *)
+  (*     destruct nck; unfold clock_of_nclock; simpl in *; *)
+  (*       match goal with H:wt_nclock _ _ |- _ => inv H end; auto. *)
+  (*   - match goal with H:Forall (wt_nclock _) _ |- _ => *)
+  (*                     rewrite Forall_map in H end. *)
+  (*     apply in_map_iff in Hin. *)
+  (*     destruct Hin as ((ty & nck) & Hck & Hin). *)
+  (*     apply Forall_forall with (1:=H3) in Hin. *)
+  (*     destruct nck; unfold clock_of_nclock in *; simpl in *; subst; *)
+  (*       match goal with H:wt_nclock _ _ |- _ => inv H end; auto. *)
+  (*   - destruct nck; unfold clock_of_nclock in *; simpl in *; *)
+  (*       apply in_map_iff in Hin; destruct Hin as (? & Hs & Hin); subst; *)
+  (*         match goal with H:wt_nclock _ _ |- _ => inv H end; auto. *)
+  (*   - destruct nck; unfold clock_of_nclock in *; simpl in *; *)
+  (*       apply in_map_iff in Hin; destruct Hin as (? & Hs & Hin); subst; *)
+  (*         match goal with H:wt_nclock _ _ |- _ => inv H end; auto. *)
+  (*   - destruct nck; unfold clock_of_nclock in *; simpl in *; *)
+  (*       apply in_map_iff in Hin; destruct Hin as (? & Hs & Hin); subst; *)
+  (*         match goal with H:wt_nclock _ _ |- _ => inv H end; auto. *)
+  (*   - apply in_map_iff in Hin. *)
+  (*     destruct Hin as (x & Hs & Hin). *)
+  (*     match goal with H:Forall _ anns |- _ => *)
+  (*                     apply Forall_forall with (1:=H) in Hin end. *)
+  (*     destruct x as (ty, nck). *)
+  (*     destruct nck; unfold clock_of_nclock in *; simpl in *; *)
+  (*       subst; match goal with H:wt_nclock _ _ |- _ => inv H end; auto. *)
+  (*   - apply in_map_iff in Hin. *)
+  (*     destruct Hin as (x & Hs & Hin). *)
+  (*     match goal with H:Forall _ anns |- _ => *)
+  (*                     apply Forall_forall with (1:=H) in Hin end. *)
+  (*     destruct x as (ty, nck). *)
+  (*     destruct nck; unfold clock_of_nclock in *; simpl in *; *)
+  (*       subst; match goal with H:wt_nclock _ _ |- _ => inv H end; auto. *)
+  (* Qed. *)
 
   (** Adding variables to the environment preserves typing *)
 
@@ -810,10 +504,14 @@ Module Type LTYPING
         intros; eauto.
       - (* app *)
         eapply Forall_impl; [| eauto].
-        intros; eauto.
+        intros; simpl in *; eauto.
+        eapply wt_nclock_incl; eauto.
+        eapply incl_appl'; eauto.
       - (* app (reset) *)
         eapply Forall_impl; [| eauto].
-        intros; eauto.
+        intros; simpl in *; eauto.
+        eapply wt_nclock_incl; eauto.
+        eapply incl_appl'; eauto.
     Qed.
 
     Lemma wt_equation_incl : forall G vars vars' eq,
@@ -831,6 +529,482 @@ Module Type LTYPING
     Qed.
 
   End incl.
+
+  (** Validation *)
+
+  Module OpAux := OperatorsAux Op.
+
+  Fixpoint check_clock (venv : Env.t type) (ck : clock) : bool :=
+    match ck with
+    | Cbase => true
+    | Con ck' x b =>
+      match Env.find x venv with
+      | None => false
+      | Some xt => (xt ==b bool_type) && check_clock venv ck'
+      end
+    end.
+
+  Definition check_nclock (venv : Env.t type) (nck : nclock) : bool :=
+    check_clock venv (fst nck).
+
+  (* TODO: Move elsewhere? *)
+  Local Ltac DestructMatch :=
+    repeat progress
+           match goal with
+           | H:match ?e with _ => _ end = _ |- _ =>
+             let Heq := fresh "Heq" in
+             destruct e eqn:Heq; try discriminate
+           end.
+
+  Lemma check_clock_correct:
+    forall venv ck,
+      check_clock venv ck = true ->
+      wt_clock (Env.elements venv) ck.
+  Proof.
+    induction ck; intro CC. now constructor.
+    simpl in CC. DestructMatch.
+    rewrite Bool.andb_true_iff in CC; destruct CC as (CC1 & CC2).
+    apply IHck in CC2. rewrite equiv_decb_equiv in CC1; inv CC1.
+    apply Env.elements_correct in Heq.
+    constructor; auto.
+  Qed.
+
+  Lemma check_nclock_correct:
+    forall venv nck,
+      check_nclock venv nck = true ->
+      wt_nclock (Env.elements venv) nck.
+  Proof.
+    destruct nck as (n, ck).
+    intro CC; now apply check_clock_correct in CC.
+  Qed.
+  Local Hint Resolve check_nclock_correct.
+
+  Section ValidateExpression.
+
+    Variable G : global.
+    Variable venv : Env.t type.
+
+    Open Scope option_monad_scope.
+
+    Definition check_paired_types (t1 t2 : type) (tc : ann) : bool :=
+      let '(t, c) := tc in
+      (t1 ==b t) && (t2 ==b t) && (check_nclock venv c).
+
+    Definition check_reset (rt : option (option (list type))) : bool :=
+      match rt with
+      | None => true
+      | Some (Some [ty]) => ty ==b bool_type
+      | _ => false
+      end.
+
+    Function check_var (x : ident) (ty : type) : bool :=
+      match Env.find x venv with
+      | None => false
+      | Some xt => ty ==b xt
+      end.
+
+    Fixpoint check_exp (e : exp) : option (list type) :=
+      match e with
+      | Econst c => Some ([type_const c])
+
+      | Evar x (xt, nck) =>
+        if check_var x xt && check_nclock venv nck then Some [xt] else None
+
+      | Eunop op e (xt, nck) =>
+        do te <- assert_singleton (check_exp e);
+        do t <- type_unop op te;
+        if (xt ==b t) && check_nclock venv nck then Some [xt] else None
+
+      | Ebinop op e1 e2 (xt, nck) =>
+        do te1 <- assert_singleton (check_exp e1);
+        do te2 <- assert_singleton (check_exp e2);
+        do t <- type_binop op te1 te2;
+        if (xt ==b t) && check_nclock venv nck then Some [xt] else None
+
+      | Efby e0s es anns =>
+        do t0s <- oconcat (map check_exp e0s);
+        do ts <- oconcat (map check_exp es);
+        if forall3b check_paired_types t0s ts anns
+        then Some (map fst anns) else None
+
+      | Ewhen es x b (tys, nck) =>
+        do ts <- oconcat (map check_exp es);
+        if check_var x bool_type && (forall2b equiv_decb ts tys) && (check_nclock venv nck)
+        then Some tys else None
+
+      | Emerge x e1s e2s (tys, nck) =>
+        do t1s <- oconcat (map check_exp e1s);
+        do t2s <- oconcat (map check_exp e2s);
+        if check_var x bool_type
+             && (forall3b equiv_decb3 t1s t2s tys)
+             && (check_nclock venv nck)
+        then Some tys else None
+
+      | Eite e e1s e2s (tys, nck) =>
+        do t1s <- oconcat (map check_exp e1s);
+        do t2s <- oconcat (map check_exp e2s);
+        do xt <- assert_singleton (check_exp e);
+        if (xt ==b bool_type)
+             && (forall3b equiv_decb3 t1s t2s tys)
+             && (check_nclock venv nck)
+        then Some tys else None
+
+      | Eapp f es ro anns =>
+        do n <- find_node f G;
+        do ts <- oconcat (map check_exp es);
+        if (forall2b (fun et '(_, (t, _)) => et ==b t) ts n.(n_in))
+             && (forall2b (fun '(ot, oc) '(_, (t, _)) =>
+                             check_nclock (Env.adds' (idty (fresh_ins es++anon_streams anns)) venv) oc
+                             && (ot ==b t)) anns n.(n_out))
+             && check_reset (option_map check_exp ro)
+        then Some (map fst anns)
+        else None
+      end.
+
+    Definition check_rhs (e : exp) : option (list type) :=
+      match e with
+      | Eapp f es ro anns =>
+        do n <- find_node f G;
+        do ts <- oconcat (map check_exp es);
+        if (forall2b (fun et '(_, (t, _)) => et ==b t) ts n.(n_in))
+             && (forall2b (fun '(ot, oc) '(_, (t, _)) =>
+                             check_nclock (Env.adds' (idty (fresh_ins es)) venv) oc
+                             && (ot ==b t)) anns n.(n_out))
+             && check_reset (option_map check_exp ro)
+        then Some (map fst anns)
+        else None
+      | e => check_exp e
+      end.
+
+    Definition check_equation (eq : equation) : bool :=
+      let '(xs, es) := eq in
+      match oconcat (map check_rhs es) with
+      | None => false
+      | Some tys => forall2b check_var xs tys
+      end.
+
+    Lemma check_var_correct:
+      forall x ty,
+        check_var x ty = true <-> In (x, ty) (Env.elements venv).
+    Proof.
+      unfold check_var. split; intros HH.
+      - DestructMatch; simpl.
+        rewrite equiv_decb_equiv in HH. inv HH.
+        take (Env.find _ _ = Some _) and apply Env.elements_correct in it; eauto.
+      - apply Env.elements_complete in HH as ->.
+        apply equiv_decb_refl.
+    Qed.
+    Local Hint Resolve check_var_correct.
+
+    Lemma check_paired_types_correct:
+      forall tys1 tys2 anns,
+        forall3b check_paired_types tys1 tys2 anns = true ->
+        tys1 = map fst anns
+        /\ tys2 = map fst anns
+        /\ Forall (wt_nclock (Env.elements venv)) (map snd anns).
+    Proof.
+      setoid_rewrite forall3b_Forall3.
+      induction 1 as [|ty1 ty2 (ty, nck) tys1 tys2 anns IH1 IH2 (? & ? & IH3)];
+        subst; simpl; eauto.
+      simpl in IH1.
+      repeat rewrite Bool.andb_true_iff in IH1.
+      setoid_rewrite equiv_decb_equiv in IH1.
+      destruct IH1 as ((-> & ->) & IH1).
+      apply check_nclock_correct in IH1. auto.
+    Qed.
+
+    Lemma oconcat_map_check_exp':
+      forall {f} es tys,
+        (forall e tys,
+            In e es ->
+            NoDupMembers (Env.elements venv++idty (fresh_in e)) ->
+            f e = Some tys ->
+            wt_exp G (Env.elements venv) e /\ typeof e = tys) ->
+        NoDupMembers (Env.elements venv++idty (fresh_ins es)) ->
+        oconcat (map f es) = Some tys ->
+        Forall (wt_exp G (Env.elements venv)) es
+        /\ typesof es = tys.
+    Proof.
+      induction es as [|e es IH]; intros tys WTf ND CE. now inv CE; auto.
+      simpl in CE. destruct (f e) eqn:Ce; [|now omonadInv CE].
+      destruct (oconcat (map f es)) as [tes|]; [|now omonadInv CE].
+      omonadInv CE. simpl.
+      apply WTf in Ce as (Ce1 & ->); auto with datatypes.
+      destruct (IH tes) as (? & ->); auto.
+      intros * Ies ND' Fe. apply WTf in Fe; auto with datatypes.
+      + unfold fresh_ins, idty in *; simpl in *. rewrite map_app in *.
+        rewrite Permutation_swap in ND. apply NoDupMembers_app_r in ND; auto.
+      + unfold fresh_ins, idty in *; simpl in *. rewrite map_app in *.
+        rewrite app_assoc in ND. apply NoDupMembers_app_l in ND; auto.
+    Qed.
+
+    Import Permutation.
+    Local Hint Constructors wt_exp.
+    Lemma check_exp_correct:
+      forall e tys,
+        NoDupMembers (Env.elements venv++(idty (fresh_in e))) ->
+        check_exp e = Some tys ->
+        wt_exp G (Env.elements venv) e
+        /\ typeof e = tys.
+    Proof with eauto.
+      induction e using exp_ind2; simpl; intros tys ND CE;
+      repeat progress
+               match goal with
+               | a:ann |- _ => destruct a
+               | a:lann |- _ => destruct a
+               | p:type * clock |- _ => destruct p
+               | H:obind _ _ = Some _ |- _ => omonadInv H
+               | H:obind2 _ _ = Some _ |- _ => omonadInv H
+               | H:obind ?v _ = Some _ |- _ =>
+                 let OE:=fresh "OE0" in destruct v eqn:OE; [simpl in H|now omonadInv H]
+               | H: _ && _ = true |- _ => apply Bool.andb_true_iff in H as (? & ?)
+               | H: ((_ ==b _) = true) |- _ => rewrite equiv_decb_equiv in H; inv H
+               | H: check_nclock _ = true |- _ => apply check_nclock_correct in H
+               | H: Env.find _ _ = Some _ |- _ => apply Env.elements_correct in H
+               | H:(obind2 (Env.find ?x ?env) _) = Some _ |- _ =>
+                 let EF := fresh "EF0" in
+                 destruct (Env.find x env) eqn:EF
+               | H:(if ?c then Some _ else None) = Some _ |- _ =>
+                 let C := fresh "C0" in
+                 destruct c eqn:C
+               | H:None = Some _ |- _ => discriminate
+               | H:Some _ = Some _ |- _ => inv H
+               | H:assert_singleton _ = Some _ |- _ => apply assert_singleton_spec in H
+               | H:check_var _ _ = true |- _ => apply check_var_correct in H
+               | H:forall3b check_paired_types ?tys1 ?tys2 ?anns = true |- _ =>
+                 apply check_paired_types_correct in H as (? & ? & ?)
+               | H:forall2b equiv_decb ?xs ?ys = true |- _ =>
+                 apply forall2b_Forall2_equiv_decb in H
+               | H:forall3b equiv_decb3 _ _ _ = true |- _ =>
+                 apply forall3b_equiv_decb3 in H as (? & ?)
+               | H:Forall2 eq _ _ |- _ => apply Forall2_eq in H
+               | H:forall2b _ _ _ = true |- _ => apply forall2b_Forall2 in H
+               end...
+
+      Ltac ndup_simpl :=
+        unfold idty in *; repeat rewrite map_app in *.
+      Ltac ndup_l H :=
+        ndup_simpl;
+        rewrite app_assoc in H; apply NoDupMembers_app_l in H; auto.
+      Ltac ndup_r H :=
+        ndup_simpl;
+        rewrite Permutation_swap in H;
+        apply NoDupMembers_app_r in H ; auto.
+
+      - (* Eunop *)
+        apply IHe in OE0 as (? & ?)...
+      - (* Ebinop *)
+        assert (NoDupMembers (Env.elements venv ++ idty (fresh_in e1))) as ND1 by ndup_l ND.
+        assert (NoDupMembers (Env.elements venv ++ idty (fresh_in e2))) as ND2 by ndup_r ND.
+        apply IHe1 in OE0 as (? & ?); apply IHe2 in OE1 as (? & ?)...
+      - (* Efby *)
+        take (Forall _ e0s) and rewrite Forall_forall in it.
+        take (Forall _ es) and rewrite Forall_forall in it.
+        apply oconcat_map_check_exp' in OE0 as (? & ?)...
+        apply oconcat_map_check_exp' in OE1 as (? & ?)...
+        subst; eauto using wt_exp.
+        + ndup_r ND.
+        + ndup_l ND.
+      - (* Ewhen *)
+        subst. take (Forall _ es) and rewrite Forall_forall in it.
+        take (oconcat (map check_exp _) = Some _) and
+             apply oconcat_map_check_exp' in it as (? & ?); eauto using wt_exp.
+      - (* Emerge *)
+        take (Forall _ ets) and rewrite Forall_forall in it.
+        take (Forall _ efs) and rewrite Forall_forall in it.
+        take (oconcat (map check_exp _) = Some _) and
+             apply oconcat_map_check_exp' in it as (? & ?); auto.
+        take (oconcat (map check_exp _) = Some _) and
+             apply oconcat_map_check_exp' in it as (? & ?); auto.
+        subst. eauto using wt_exp.
+        + ndup_l ND.
+        + ndup_r ND.
+      - (* Eite *)
+        take (check_exp _ = Some _) and apply IHe in it as (? & ?).
+        take (Forall _ ets) and rewrite Forall_forall in it.
+        take (Forall _ efs) and rewrite Forall_forall in it.
+        take (oconcat (map check_exp _) = Some _) and
+             apply oconcat_map_check_exp' in it as (? & ?); auto.
+        take (oconcat (map check_exp _) = Some _) and
+             apply oconcat_map_check_exp' in it as (? & ?); auto.
+        subst. eauto using wt_exp.
+        + ndup_simpl.
+          rewrite Permutation_swap in ND.
+          rewrite app_assoc in ND. apply NoDupMembers_app_l in ND; auto.
+        + ndup_simpl.
+          rewrite Permutation.Permutation_app_comm in ND.
+          repeat rewrite <- app_assoc in ND.
+          apply NoDupMembers_app_r in ND. apply NoDupMembers_app_r in ND.
+          rewrite Permutation.Permutation_app_comm in ND. assumption.
+        + ndup_simpl.
+          rewrite app_assoc in ND. apply NoDupMembers_app_l in ND; auto.
+      - (* Eapp *)
+        take (Forall _ es) and rewrite Forall_forall in it.
+        take (oconcat (map check_exp _) = Some _) and
+             apply oconcat_map_check_exp' in it as (? & ?); auto.
+        2: { destruct ro; ndup_simpl.
+             + repeat rewrite app_assoc in ND.
+               apply NoDupMembers_app_l in ND. apply NoDupMembers_app_l in ND.
+               assumption.
+             + rewrite app_assoc in ND.
+               apply NoDupMembers_app_l in ND.
+               assumption.
+        }
+        split; auto. subst.
+        assert (Forall2 (fun et '(_, (t, _)) => et = t) (typesof es) n.(n_in)).
+        { take (Forall2 _ (typesof es) n.(n_in))
+               and apply Forall2_impl_In with (2:=it).
+          intros ? (? & (? & ?)) ? ? EQ.
+          now rewrite equiv_decb_equiv in EQ. }
+        assert (Forall2 (fun ann '(_, (t, _)) => fst ann = t) a n.(n_out)).
+        { take (Forall2 _ _ n.(n_out)) and apply Forall2_impl_In with (2:=it).
+          intros (? & ?) (? & (? & ?)) ? ? EQ.
+          apply Bool.andb_true_iff in EQ as (EQ1 & EQ2).
+          now rewrite equiv_decb_equiv in EQ2. }
+        assert (Forall (fun ann => wt_nclock ((Env.elements venv)++idty (fresh_ins es++anon_streams a)) (snd ann)) a).
+        { repeat take (Forall2 _ _ n.(n_out)) and apply Forall2_ignore2 in it.
+          apply Forall_impl_In with (2:=it).
+          intros (? & ?) ? ((? & (? & ?)) & (? & EQ)); simpl.
+          apply Bool.andb_true_iff in EQ as (EQ1 & EQ2).
+          apply check_nclock_correct in EQ1. rewrite Env.elements_adds in EQ1; auto.
+          destruct ro; auto.
+          ndup_simpl.
+          rewrite app_assoc in ND.
+          rewrite Permutation_app_comm in ND.
+          rewrite <- app_assoc in ND. apply NoDupMembers_app_r in ND.
+          rewrite Permutation_app_comm in ND.
+          rewrite <- app_assoc in ND; auto.
+        }
+        destruct ro; econstructor; eauto; simpl in *;
+          clear it; DestructMatch; subst;
+            destruct (H [t]) as [CE1 CE2]; auto.
+        + ndup_simpl.
+          repeat rewrite app_assoc in ND.
+          apply NoDupMembers_app_l in ND.
+          repeat rewrite <- app_assoc in ND.
+          rewrite Permutation_swap in ND.
+          apply NoDupMembers_app_r in ND; auto.
+        + ndup_simpl.
+          repeat rewrite app_assoc in ND.
+          apply NoDupMembers_app_l in ND.
+          repeat rewrite <- app_assoc in ND.
+          rewrite Permutation_swap in ND.
+          apply NoDupMembers_app_r in ND; auto.
+        + rewrite equiv_decb_equiv in H2. congruence.
+    Qed.
+
+    Corollary oconcat_map_check_exp:
+      forall es tys,
+        NoDupMembers (Env.elements venv++idty (fresh_ins es)) ->
+        oconcat (map check_exp es) = Some tys ->
+        Forall (wt_exp G (Env.elements venv)) es
+        /\ typesof es = tys.
+    Proof.
+      intros.
+      eapply oconcat_map_check_exp'; eauto.
+      intros. eapply check_exp_correct; eauto.
+    Qed.
+
+    Lemma check_rhs_correct:
+      forall e tys,
+        NoDupMembers (Env.elements venv++(idty (anon_in e))) -> (* Should be anon_in ? *)
+        check_rhs e = Some tys ->
+        wt_exp G (Env.elements venv) e
+        /\ typeof e = tys.
+    Proof with eauto.
+      intros e tys ND CR.
+      destruct e; try (now apply check_exp_correct).
+      simpl in CR.
+
+      repeat progress
+               match goal with
+               | H:obind ?v _ = Some _ |- _ =>
+                 let OE:=fresh "OE0" in destruct v eqn:OE; [simpl in H|now omonadInv H]
+               | H: _ && _ = true |- _ => apply Bool.andb_true_iff in H as (? & ?)
+               | H: ((_ ==b _) = true) |- _ => rewrite equiv_decb_equiv in H; inv H
+               | H: check_nclock _ = true |- _ => apply check_nclock_correct in H
+               | H: Env.find _ _ = Some _ |- _ => apply Env.elements_correct in H
+               | H:(if ?c then Some _ else None) = Some _ |- _ =>
+                 let C := fresh "C0" in
+                 destruct c eqn:C
+               | H:None = Some _ |- _ => discriminate
+               | H:Some _ = Some _ |- _ => inv H
+               | H:forall2b _ _ _ = true |- _ => apply forall2b_Forall2 in H
+               end...
+      split...
+
+      simpl in ND.
+      take (oconcat (map check_exp _) = Some _) and
+           apply oconcat_map_check_exp in it as (? & ?); auto.
+      2: { destruct o; ndup_simpl...
+           rewrite app_assoc in ND.
+           apply NoDupMembers_app_l in ND... }
+      subst.
+      assert (Forall2 (fun et '(_, (t, _)) => et = t) (typesof l) n.(n_in)).
+        { take (Forall2 _ (typesof l) n.(n_in))
+               and apply Forall2_impl_In with (2:=it).
+          intros ? (? & (? & ?)) ? ? EQ.
+          now rewrite equiv_decb_equiv in EQ. }
+        assert (Forall2 (fun ann '(_, (t, _)) => fst ann = t) l0 n.(n_out)).
+        { take (Forall2 _ _ n.(n_out)) and apply Forall2_impl_In with (2:=it).
+          intros (? & ?) (? & (? & ?)) ? ? EQ.
+          apply Bool.andb_true_iff in EQ as (EQ1 & EQ2).
+          now rewrite equiv_decb_equiv in EQ2. }
+        assert (Forall (fun a => wt_nclock (Env.elements venv ++ idty (fresh_ins l++anon_streams l0)) (snd a)) l0).
+        { repeat take (Forall2 _ _ n.(n_out)) and apply Forall2_ignore2 in it.
+          apply Forall_impl_In with (2:=it).
+          intros (? & ?) ? ((? & (? & ?)) & (? & EQ)); simpl.
+          apply Bool.andb_true_iff in EQ as (EQ1 & EQ2).
+          unfold idty in *; rewrite map_app in *.
+          apply check_nclock_correct in EQ1. rewrite Env.elements_adds in EQ1; auto.
+          + eapply wt_nclock_incl; eauto. apply incl_appr'.
+            eapply incl_appl. reflexivity.
+          + destruct o; auto.
+            rewrite map_app in ND. rewrite app_assoc in ND.
+            apply NoDupMembers_app_l in ND. assumption. }
+        destruct o; simpl in H0; DestructMatch; econstructor...
+        1,2:(apply check_exp_correct in Heq as [Hwt Heq]; eauto).
+        1,3:unfold idty in *; rewrite map_app in *; rewrite Permutation_swap in ND; apply NoDupMembers_app_r in ND; auto.
+        rewrite equiv_decb_equiv in H0. congruence.
+    Qed.
+
+    Corollary oconcat_map_check_rhs:
+      forall es tys,
+        NoDupMembers (Env.elements venv++idty (anon_ins es)) ->
+        oconcat (map check_rhs es) = Some tys ->
+        Forall (wt_exp G (Env.elements venv)) es
+        /\ typesof es = tys.
+    Proof.
+      induction es as [|e es IH]; intros tys ND CE. now inv CE; auto.
+      simpl in CE. destruct (check_rhs e) eqn:Ce; [|now omonadInv CE].
+      destruct (oconcat (map check_rhs es)) as [tes|]; [|now omonadInv CE].
+      omonadInv CE. simpl.
+      apply check_rhs_correct in Ce as (Ce1 & ->); auto with datatypes.
+      destruct (IH tes) as (? & ->); auto.
+      + unfold anon_ins, idty in *; simpl in *. rewrite map_app in *.
+        rewrite Permutation_swap in ND. apply NoDupMembers_app_r in ND; auto.
+      + unfold anon_ins, idty in *; simpl in *. rewrite map_app in *.
+        rewrite app_assoc in ND. apply NoDupMembers_app_l in ND; auto.
+    Qed.
+
+    Lemma check_equation_correct:
+      forall eq,
+        NoDupMembers (Env.elements venv++(idty (anon_in_eq eq))) ->
+        check_equation eq = true ->
+        wt_equation G (Env.elements venv) eq.
+    Proof.
+      intros eq ND CE. destruct eq as (xs, es); simpl in CE.
+      DestructMatch.
+      take (oconcat (map check_rhs _) = Some _)
+           and apply oconcat_map_check_rhs in it as (? & ?).
+      take (forall2b check_var _ _ = true)
+           and apply forall2b_Forall2 in it.
+      setoid_rewrite check_var_correct in it.
+      subst; constructor; auto.
+      unfold anon_in_eq in ND; auto.
+    Qed.
+
+  End ValidateExpression.
 
   Section interface_eq.
 
